Remove the sorries from Primitives.lean

backends/lean/Primitives.lean
@@ -2,9 +2,10 @@ import Lean
 import Lean.Meta.Tactic.Simp
 import Init.Data.List.Basic
 import Mathlib.Tactic.RunCmd
+import Mathlib.Tactic.Linarith
 
 --------------------
--- ASSERT COMMAND --
+-- ASSERT COMMAND --Std.
 --------------------
 
 open Lean Elab Command Term Meta
@@ -249,27 +250,53 @@ def Scalar.cMax (ty : ScalarTy) : Int :=
   | .Usize => U32.max
   | _ => Scalar.max ty
 
-theorem Scalar.cMin_bound ty : Scalar.min ty <= Scalar.cMin ty := by sorry
-theorem Scalar.cMax_bound ty : Scalar.min ty <= Scalar.cMin ty := by sorry
+theorem Scalar.cMin_bound ty : Scalar.min ty ≤ Scalar.cMin ty := by
+  cases ty <;> simp [Scalar.min, Scalar.max, Scalar.cMin, Scalar.cMax] at *
+  cases System.Platform.numBits_eq <;>
+  unfold System.Platform.numBits at * <;>
+  simp [*]
+
+theorem Scalar.cMax_bound ty : Scalar.cMax ty ≤ Scalar.max ty := by
+  cases ty <;> simp [Scalar.min, Scalar.max, Scalar.cMin, Scalar.cMax] at * <;>
+  cases System.Platform.numBits_eq <;>
+  unfold System.Platform.numBits at * <;>
+  simp [*]
+
+theorem Scalar.cMin_suffices ty (h : Scalar.cMin ty ≤ x) : Scalar.min ty ≤ x := by
+  cases ty <;> simp [Scalar.min, Scalar.max, Scalar.cMin, Scalar.cMax] at * <;>
+  cases System.Platform.numBits_eq <;>
+  unfold System.Platform.numBits at * <;>
+  simp [*] at *
+  -- TODO: I would have expected terms like `-(1 + 1) ^ 63` to be simplified
+  linarith
+
+theorem Scalar.cMax_suffices ty (h : x ≤ Scalar.cMax ty) : x ≤ Scalar.max ty := by
+  cases ty <;> simp [Scalar.min, Scalar.max, Scalar.cMin, Scalar.cMax] at * <;>
+  cases System.Platform.numBits_eq <;>
+  unfold System.Platform.numBits at * <;>
+  simp [*] at * <;>
+  -- TODO: I would have expected terms like `-(1 + 1) ^ 63` to be simplified
+  linarith
 
 structure Scalar (ty : ScalarTy) where
   val : Int
-  hmin : Scalar.min ty <= val
-  hmax : val <= Scalar.max ty
+  hmin : Scalar.min ty ≤ val
+  hmax : val ≤ Scalar.max ty
 
 theorem Scalar.bound_suffices (ty : ScalarTy) (x : Int) :
-  Scalar.cMin ty <= x && x <= Scalar.cMax ty ->
-  (decide (Scalar.min ty ≤ x) && decide (x ≤ Scalar.max ty)) = true
-  := by sorry
+  Scalar.cMin ty ≤ x ∧ x ≤ Scalar.cMax ty ->
+  Scalar.min ty ≤ x ∧ x ≤ Scalar.max ty
+  :=
+  λ h => by
+  apply And.intro <;> have hmin := Scalar.cMin_bound ty <;> have hmax := Scalar.cMax_bound ty <;> linarith
 
 def Scalar.ofIntCore {ty : ScalarTy} (x : Int)
-  (hmin : Scalar.min ty <= x) (hmax : x <= Scalar.max ty) : Scalar ty :=
+  (hmin : Scalar.min ty ≤ x) (hmax : x ≤ Scalar.max ty) : Scalar ty :=
   { val := x, hmin := hmin, hmax := hmax }
 
 def Scalar.ofInt {ty : ScalarTy} (x : Int)
-  (h : Scalar.min ty <= x && x <= Scalar.max ty) : Scalar ty :=
-  let hmin: Scalar.min ty <= x := by sorry
-  let hmax: x <= Scalar.max ty := by sorry
+  (h : Scalar.min ty ≤ x ∧ x ≤ Scalar.max ty) : Scalar ty :=
+  let ⟨ hmin, hmax ⟩ := h
   Scalar.ofIntCore x hmin hmax
 
 -- Further thoughts: look at what has been done here:
@@ -279,12 +306,15 @@ def Scalar.ofInt {ty : ScalarTy} (x : Int)
 -- which both contain a fair amount of reasoning already!
 def Scalar.tryMk (ty : ScalarTy) (x : Int) : Result (Scalar ty) :=
   -- TODO: write this with only one if then else
-  if hmin_cons: Scalar.cMin ty <= x || Scalar.min ty <= x then
-    if hmax_cons: x <= Scalar.cMax ty || x <= Scalar.max ty then
-      let hmin: Scalar.min ty <= x := by sorry
-      let hmax: x <= Scalar.max ty := by sorry
-      return Scalar.ofIntCore x hmin hmax
-    else fail integerOverflow
+  if h: (Scalar.cMin ty ≤ x || Scalar.min ty ≤ x) && (x ≤ Scalar.cMax ty || x ≤ Scalar.max ty) then
+    let h: Scalar.min ty ≤ x ∧ x ≤ Scalar.max ty := by
+      simp at *
+      have ⟨ hmin, hmax ⟩ := h
+      have hbmin := Scalar.cMin_bound ty
+      have hbmax := Scalar.cMax_bound ty
+      cases hmin <;> cases hmax <;> apply And.intro <;> linarith
+    let ⟨ hmin, hmax ⟩ := h
+    return Scalar.ofIntCore x hmin hmax
   else fail integerOverflow
 
 def Scalar.neg {ty : ScalarTy} (x : Scalar ty) : Result (Scalar ty) := Scalar.tryMk ty (- x.val)
@@ -292,11 +322,39 @@ def Scalar.neg {ty : ScalarTy} (x : Scalar ty) : Result (Scalar ty) := Scalar.tr
 def Scalar.div {ty : ScalarTy} (x : Scalar ty) (y : Scalar ty) : Result (Scalar ty) :=
   if y.val != 0 then Scalar.tryMk ty (x.val / y.val) else fail divisionByZero
 
--- Checking that the % operation in Lean computes the same as the remainder operation in Rust
-#assert 1 % 2 = (1:Int)
-#assert (-1) % 2 = -1
-#assert 1 % (-2) = 1
-#assert (-1) % (-2) = -1
+-- Our custom remainder operation, which satisfies the semantics of Rust
+-- TODO: is there a better way?
+def scalar_rem (x y : Int) : Int :=
+  if 0 ≤ x then |x| % |y|
+  else - (|x| % |y|)
+
+-- Our custom division operation, which satisfies the semantics of Rust
+-- TODO: is there a better way?
+def scalar_div (x y : Int) : Int :=
+  if 0 ≤ x && 0 ≤ y then |x| / |y|
+  else if 0 ≤ x && y < 0 then - (|x| / |y|)
+  else if x < 0 && 0 ≤ y then - (|x| / |y|)
+  else |x| / |y|
+
+-- Checking that the remainder operation is correct
+#assert scalar_rem 1 2 = 1
+#assert scalar_rem (-1) 2 = -1
+#assert scalar_rem 1 (-2) = 1
+#assert scalar_rem (-1) (-2) = -1
+#assert scalar_rem 7 3 = (1:Int)
+#assert scalar_rem (-7) 3 = -1
+#assert scalar_rem 7 (-3) = 1
+#assert scalar_rem (-7) (-3) = -1
+
+-- Checking that the division operation is correct
+#assert scalar_div 3 2 = 1
+#assert scalar_div (-3) 2 = -1
+#assert scalar_div 3 (-2) = -1
+#assert scalar_div (-3) (-2) = 1
+#assert scalar_div 7 3 = 2
+#assert scalar_div (-7) 3 = -2
+#assert scalar_div 7 (-3) = -2
+#assert scalar_div (-7) (-3) = 2
 
 def Scalar.rem {ty : ScalarTy} (x : Scalar ty) (y : Scalar ty) : Result (Scalar ty) :=
   if y.val != 0 then Scalar.tryMk ty (x.val % y.val) else fail divisionByZero
@@ -479,20 +537,29 @@ macro_rules
 -- VECTORS --
 -------------
 
-def Vec (α : Type u) := { l : List α // List.length l <= Usize.max }
+def Vec (α : Type u) := { l : List α // List.length l ≤ Usize.max }
 
-def vec_new (α : Type u): Vec α := ⟨ [], by sorry ⟩
+def vec_new (α : Type u): Vec α := ⟨ [], by apply Scalar.cMax_suffices .Usize; simp ⟩
 
 def vec_len (α : Type u) (v : Vec α) : Usize :=
   let ⟨ v, l ⟩ := v
-  Usize.ofIntCore (List.length v) (by sorry) l
+  Usize.ofIntCore (List.length v) (by simp [Scalar.min]) l
  
 def vec_push_fwd (α : Type u) (_ : Vec α) (_ : α) : Unit := ()
 
 def vec_push_back (α : Type u) (v : Vec α) (x : α) : Result (Vec α)
   :=
-  if h : List.length v.val <= U32.max || List.length v.val <= Usize.max then
-    return ⟨ List.concat v.val x, by sorry ⟩
+  let nlen := List.length v.val + 1
+  if h : nlen ≤ U32.max || nlen ≤ Usize.max then
+    have h : nlen ≤ Usize.max := by
+      simp at *
+      cases System.Platform.numBits_eq <;>
+      unfold System.Platform.numBits at * <;>
+      simp [*] at * <;>
+      try assumption
+      cases h <;>
+      linarith
+    return ⟨ List.concat v.val x, by simp at *; assumption ⟩
   else
     fail maximumSizeExceeded
 
@@ -506,30 +573,28 @@ def vec_insert_back (α : Type u) (v: Vec α) (i: Usize) (x: α): Result (Vec α
   if i.val < List.length v.val then
     -- TODO: maybe we should redefine a list library which uses integers
     -- (instead of natural numbers)
-    let i : Nat :=
-      match i.val with
-      | .ofNat n => n
-      | .negSucc n => by sorry -- TODO: we can't get here
-    let isLt: i < USize.size := by sorry
-    let i : Fin USize.size := { val := i, isLt := isLt }
-    .ret ⟨ List.set v.val i.val x, by
-      have h: List.length v.val <= Usize.max := v.property
-      rewrite [ List.length_set v.val i.val x ]
+    let i := i.val.toNat
+    .ret ⟨ List.set v.val i x, by
+      have h: List.length v.val ≤ Usize.max := v.property
+      simp [*] at *
       assumption
     ⟩
   else
     .fail arrayOutOfBounds
 
+def vec_index_to_fin {α : Type u} {v: Vec α} {i: Usize} (h : i.val < List.length v.val) :
+  Fin (List.length v.val) :=
+  let j := i.val.toNat
+  let h: j < List.length v.val := by
+    have heq := @Int.toNat_lt (List.length v.val) i.val i.hmin
+    apply heq.mpr
+    assumption
+  ⟨j, h⟩
+
 def vec_index_fwd (α : Type u) (v: Vec α) (i: Usize): Result α :=
-  if i.val < List.length v.val then
-    let i : Nat :=
-      match i.val with
-      | .ofNat n => n
-      | .negSucc n => by sorry -- TODO: we can't get here
-    let isLt: i < USize.size := by sorry
-    let i : Fin USize.size := { val := i, isLt := isLt }
-    let h: i < List.length v.val := by sorry
-    .ret (List.get v.val ⟨i.val, h⟩)
+  if h: i.val < List.length v.val then
+    let i := vec_index_to_fin h
+    .ret (List.get v.val i)
   else
     .fail arrayOutOfBounds
 
@@ -540,29 +605,18 @@ def vec_index_back (α : Type u) (v: Vec α) (i: Usize) (_: α): Result Unit :=
     .fail arrayOutOfBounds
 
 def vec_index_mut_fwd (α : Type u) (v: Vec α) (i: Usize): Result α :=
-  if i.val < List.length v.val then
-    let i : Nat :=
-      match i.val with
-      | .ofNat n => n
-      | .negSucc n => by sorry -- TODO: we can't get here
-    let isLt: i < USize.size := by sorry
-    let i : Fin USize.size := { val := i, isLt := isLt }
-    let h: i < List.length v.val := by sorry
-    .ret (List.get v.val ⟨i.val, h⟩)
+  if h: i.val < List.length v.val then
+    let i := vec_index_to_fin h
+    .ret (List.get v.val i)
   else
     .fail arrayOutOfBounds
 
 def vec_index_mut_back (α : Type u) (v: Vec α) (i: Usize) (x: α): Result (Vec α) :=
-  if i.val < List.length v.val then
-    let i : Nat :=
-      match i.val with
-      | .ofNat n => n
-      | .negSucc n => by sorry -- TODO: we can't get here
-    let isLt: i < USize.size := by sorry
-    let i : Fin USize.size := { val := i, isLt := isLt }
-    .ret ⟨ List.set v.val i.val x, by
-      have h: List.length v.val <= Usize.max := v.property
-      rewrite [ List.length_set v.val i.val x ]
+  if h: i.val < List.length v.val then
+    let i := vec_index_to_fin h
+    .ret ⟨ List.set v.val i x, by
+      have h: List.length v.val ≤ Usize.max := v.property
+      simp [*] at *
       assumption
     ⟩
   else
