backends/lean/lakefile.lean
@@ -1,6 +1,7 @@
 import Lake
 open Lake DSL
 
+-- Important: mathlib imports std4 and quote4: we mustn't add a `require std4` line
 require mathlib from git
   "https://github.com/leanprover-community/mathlib4.git"
 
